MESI: added [InvObjOwned] in [InvExcl]

src/Ex/Mesi/MesiInvExcl.v
@@ -19,20 +19,27 @@ Local Open Scope fmap.
 
 Existing Instance Mesi.ImplOStateIfc.
 
-Definition ObjsInvalid (eidx: IdxT) (oss: OStates) (msgs: MessagePool Msg) :=
+Definition ObjsInvalid (inP: IdxT -> Prop) (oss: OStates) (msgs: MessagePool Msg) :=
   forall oidx,
-    oidx <> eidx ->
+    inP oidx ->
     ost <+- oss@[oidx]; ObjInvalid oidx ost msgs.
 
-Definition InvObjExcl0 (oidx: IdxT) (ost: OState) (oss: OStates)
+Definition InvObjExcl0 (eidx: IdxT) (ost: OState) (oss: OStates)
            (msgs: MessagePool Msg) :=
-  ObjExcl0 oidx ost msgs ->
-  ObjsInvalid oidx oss msgs /\ NoCohMsgs oidx msgs.
+  ObjExcl0 eidx ost msgs ->
+  ObjsInvalid (fun oidx => eidx <> oidx) oss msgs /\
+  NoCohMsgs eidx msgs.
 
-Definition InvExcl (st: MState): Prop :=
+Definition InvObjOwned (topo: DTree) (eidx: IdxT) (eost: OState) (oss: OStates)
+           (msgs: MessagePool Msg) :=
+  eost#[owned] = true ->
+  ObjsInvalid (fun oidx => ~ In oidx (subtreeIndsOf topo eidx)) oss msgs.
+
+Definition InvExcl (topo: DTree) (st: MState): Prop :=
   forall eidx,
     eost <+- (bst_oss st)@[eidx];
-      InvObjExcl0 eidx eost (bst_oss st) (bst_msgs st).
+      (InvObjExcl0 eidx eost (bst_oss st) (bst_msgs st) /\
+       InvObjOwned topo eidx eost (bst_oss st) (bst_msgs st)).
 
 Section Facts.
 
@@ -119,20 +126,21 @@ Section Facts.
     intro Hx; dest_in; auto.
   Qed.
 
-  Ltac disc_ObjExcl0_msgs H :=
-    repeat
-      (first [apply ObjExcl0_enqMP_inv in H
-             |apply ObjExcl0_enqMsgs_inv in H
-             |apply ObjExcl0_other_midx_deqMP_inv in H; [|solve_chn_neq]
-             |apply ObjExcl0_other_midx_deqMsgs_inv in H;
-              [|eassumption|eassumption|] (** FIXME: need to debug when not working *)
-             |eapply ObjExcl0_other_msg_id_deqMP_inv in H;
-              [|eassumption|congruence]
-             |eapply ObjExcl0_other_msg_id_deqMsgs_inv in H;
-              [|eassumption|eassumption|] (** FIXME: need to debug when not working *)
-      ]).
-
 End Facts.
+
+Ltac disc_ObjExcl0_msgs H :=
+  repeat
+    (first [apply ObjExcl0_enqMP_inv in H
+           |apply ObjExcl0_enqMsgs_inv in H
+           |apply ObjExcl0_other_midx_deqMP_inv in H;
+            [|solve_chn_neq; fail]
+           |apply ObjExcl0_other_midx_deqMsgs_inv in H;
+            [|eassumption|eassumption|] (** FIXME: need to debug when not working *)
+           |eapply ObjExcl0_other_msg_id_deqMP_inv in H;
+            [|eassumption|congruence]
+           |eapply ObjExcl0_other_msg_id_deqMsgs_inv in H;
+            [|eassumption|eassumption|] (** FIXME: need to debug when not working *)
+    ]).
 
 Section InvExcl.
   Variable (tr: tree).
@@ -143,66 +151,141 @@ Section InvExcl.
   Let impl: System := impl Htr.
 
   Lemma mesi_InvExcl_init:
-    Invariant.InvInit impl InvExcl.
+    Invariant.InvInit impl (InvExcl topo).
   Proof.
     do 2 (red; simpl); intros.
     destruct (implOStatesInit tr)@[eidx] as [eost|] eqn:Heost; simpl; auto.
-    red; intros.
-    red in H; dest.
+    split.
 
-    destruct (in_dec idx_dec eidx (c_li_indices cifc ++ c_l1_indices cifc)).
-    - subst cifc; rewrite c_li_indices_head_rootOf in i by assumption.
-      inv i.
-      + split.
+    - red; intros.
+      red in H; dest.
+      destruct (in_dec idx_dec eidx (c_li_indices cifc ++ c_l1_indices cifc)).
+      + subst cifc; rewrite c_li_indices_head_rootOf in i by assumption.
+        inv i.
+        * split.
+          { red; intros.
+            destruct (implOStatesInit tr)@[oidx] as [ost|] eqn:Host; simpl; auto.
+            red.
+            destruct (in_dec idx_dec oidx ((c_li_indices (snd (tree2Topo tr 0)))
+                                             ++ c_l1_indices (snd (tree2Topo tr 0)))).
+            { rewrite c_li_indices_head_rootOf in i by assumption.
+              inv i; [exfalso; auto|].
+              rewrite implOStatesInit_value_non_root in Host by assumption.
+              inv Host.
+              left; repeat split; [simpl; solve_mesi..|].
+              do 3 red; intros; do 2 red in H3; dest_in.
+            }
+            { rewrite implOStatesInit_None in Host by assumption.
+              discriminate.
+            }
+          }
+          { do 3 red; intros; do 2 red in H1; dest_in. }
+        * exfalso.
+          rewrite implOStatesInit_value_non_root in Heost by assumption.
+          inv Heost.
+          simpl in *; solve_mesi.
+      + exfalso.
+        rewrite implOStatesInit_None in Heost by assumption.
+        discriminate.
+
+    - red; intros.
+      destruct (in_dec idx_dec eidx (c_li_indices cifc ++ c_l1_indices cifc)).
+      + subst cifc; rewrite c_li_indices_head_rootOf in i by assumption.
+        inv i.
         * red; intros.
           destruct (implOStatesInit tr)@[oidx] as [ost|] eqn:Host; simpl; auto.
           red.
           destruct (in_dec idx_dec oidx ((c_li_indices (snd (tree2Topo tr 0)))
                                            ++ c_l1_indices (snd (tree2Topo tr 0)))).
           { rewrite c_li_indices_head_rootOf in i by assumption.
-            inv i; [exfalso; auto|].
-            rewrite implOStatesInit_value_non_root in Host by assumption.
-            inv Host.
-            left; repeat split; [simpl; solve_mesi..|].
-            do 3 red; intros; do 2 red in H3; dest_in.
+            inv i.
+            { elim H0.
+              apply subtreeIndsOf_root_in.
+              { apply tree2Topo_WfDTree. }
+              { apply Subtree_refl. }
+            }
+            { rewrite implOStatesInit_value_non_root in Host by assumption.
+              inv Host.
+              left; repeat split; [simpl; solve_mesi..|].
+              do 3 red; intros; do 2 red in H2; dest_in.
+            }
           }
-          { rewrite implOStatesInit_None in Host by assumption.
-            discriminate.
-          }
-        * do 3 red; intros; do 2 red in H1; dest_in.
-      + exfalso.
-        rewrite implOStatesInit_value_non_root in Heost by assumption.
-        inv Heost.
-        simpl in *; solve_mesi.
-    - exfalso.
-      rewrite implOStatesInit_None in Heost by assumption.
-      discriminate.
+          { rewrite implOStatesInit_None in Host by assumption; discriminate. }
+        * rewrite implOStatesInit_value_non_root in Heost by assumption.
+          inv Heost; discriminate.
+      + rewrite implOStatesInit_None in Heost by assumption; discriminate.
   Qed.
 
   Lemma mesi_InvExcl_ext_in:
     forall oss orqs msgs,
-      InvExcl {| bst_oss := oss; bst_orqs := orqs; bst_msgs := msgs |} ->
+      InvExcl topo {| bst_oss := oss; bst_orqs := orqs; bst_msgs := msgs |} ->
       InObjInds tr 0 {| bst_oss := oss; bst_orqs := orqs; bst_msgs := msgs |} ->
       forall eins,
         ValidMsgsExtIn impl eins ->
-        InvExcl {| bst_oss := oss; bst_orqs := orqs; bst_msgs := enqMsgs eins msgs |}.
+        InvExcl topo {| bst_oss := oss;
+                        bst_orqs := orqs;
+                        bst_msgs := enqMsgs eins msgs |}.
   Proof.
     red; simpl; intros.
     specialize (H eidx); simpl in H.
     destruct (oss@[eidx]) as [eost|] eqn:Heost; simpl in *; auto.
-    red; intros.
+    dest; split.
 
-    destruct H2.
-    apply MsgsP_enqMsgs_inv in H3.
-    specialize (H (conj H2 H3)); dest.
+    - clear H2.
+      red; intros.
+      destruct H2.
+      apply MsgsP_enqMsgs_inv in H3.
+      specialize (H (conj H2 H3)); dest.
 
-    split.
-    - red; intros.
-      specialize (H _ H5).
+      split.
+      + red; intros.
+        specialize (H _ H5).
+        destruct (oss@[oidx]) as [ost|] eqn:Host; simpl in *; auto.
+        destruct H.
+        * left.
+          red in H; dest.
+          repeat split; [assumption..|].
+          apply MsgsP_other_midx_enqMsgs; [assumption|].
+          destruct H1; simpl.
+          eapply DisjList_SubList; [eassumption|].
+          eapply DisjList_comm, DisjList_SubList.
+          { eapply SubList_trans;
+              [|eapply tree2Topo_obj_chns_minds_SubList with (oidx:= oidx)].
+            { solve_SubList. }
+            { specialize (H0 oidx); simpl in H0.
+              rewrite Host in H0; simpl in H0.
+              eassumption.
+            }
+          }
+          { apply tree2Topo_minds_merqs_disj. }
+        * right.
+          destruct H as [idm ?]; dest.
+          exists idm; split; [|assumption].
+          apply InMP_or_enqMsgs; auto.
+
+      + apply MsgsP_other_midx_enqMsgs; [assumption|].
+        destruct H1; simpl.
+        eapply DisjList_SubList; [eassumption|].
+        eapply DisjList_comm, DisjList_SubList.
+        * eapply SubList_trans;
+            [|eapply tree2Topo_obj_chns_minds_SubList with (oidx:= eidx)].
+          { solve_SubList. }
+          { specialize (H0 eidx); simpl in H0.
+            rewrite Heost in H0; simpl in H0.
+            eassumption.
+          }
+        * apply tree2Topo_minds_merqs_disj.
+
+    - clear H.
+      red; intros.
+      specialize (H2 H).
+
+      red; intros.
+      specialize (H2 _ H3).
       destruct (oss@[oidx]) as [ost|] eqn:Host; simpl in *; auto.
-      destruct H.
+      destruct H2.
       + left.
-        red in H; dest.
+        red in H2; dest.
         repeat split; [assumption..|].
         apply MsgsP_other_midx_enqMsgs; [assumption|].
         destruct H1; simpl.
@@ -217,24 +300,12 @@ Section InvExcl.
           }
         * apply tree2Topo_minds_merqs_disj.
       + right.
-        destruct H as [idm ?]; dest.
+        destruct H2 as [idm ?]; dest.
         exists idm; split; [|assumption].
         apply InMP_or_enqMsgs; auto.
-
-    - apply MsgsP_other_midx_enqMsgs; [assumption|].
-      destruct H1; simpl.
-      eapply DisjList_SubList; [eassumption|].
-      eapply DisjList_comm, DisjList_SubList.
-      + eapply SubList_trans;
-          [|eapply tree2Topo_obj_chns_minds_SubList with (oidx:= eidx)].
-        * solve_SubList.
-        * specialize (H0 eidx); simpl in H0.
-          rewrite Heost in H0; simpl in H0.
-          eassumption.
-      + apply tree2Topo_minds_merqs_disj.
   Qed.
 
-  Corollary mesi_InvExcl_InvTrsIns: InvTrsIns impl InvExcl.
+  Corollary mesi_InvExcl_InvTrsIns: InvTrsIns impl (InvExcl topo).
   Proof.
     red; intros.
     inv H1.
@@ -244,64 +315,99 @@ Section InvExcl.
 
   Lemma mesi_InvExcl_ext_out:
     forall oss orqs msgs,
-      InvExcl {| bst_oss := oss; bst_orqs := orqs; bst_msgs := msgs |} ->
+      InvExcl topo {| bst_oss := oss; bst_orqs := orqs; bst_msgs := msgs |} ->
       InObjInds tr 0 {| bst_oss := oss; bst_orqs := orqs; bst_msgs := msgs |} ->
       forall (eouts: list (Id Msg)),
         ValidMsgsExtOut impl eouts ->
-        InvExcl {| bst_oss := oss;
-                   bst_orqs := orqs;
-                   bst_msgs := deqMsgs (idsOf eouts) msgs |}.
+        InvExcl topo {| bst_oss := oss;
+                        bst_orqs := orqs;
+                        bst_msgs := deqMsgs (idsOf eouts) msgs |}.
   Proof.
     red; simpl; intros.
     specialize (H eidx); simpl in H.
     destruct (oss@[eidx]) as [eost|] eqn:Heost; simpl in *; auto.
-    red; intros.
+    dest; split.
 
-    destruct H2.
-    apply MsgsP_other_midx_deqMsgs_inv in H3.
-    - specialize (H (conj H2 H3)); dest.
-      split.
-      + red; intros.
-        specialize (H _ H5).
-        destruct (oss@[oidx]) as [ost|] eqn:Host; simpl in *; auto.
-        destruct H.
-        * left.
-          red in H; dest.
-          repeat split; [assumption..|].
-          apply MsgsP_deqMsgs; assumption.
-        * right.
-          destruct H as [idm ?]; dest.
-          exists idm; split; [|assumption].
-          apply deqMsgs_InMP_midx; [assumption|].
-          destruct H1.
-          eapply DisjList_In_1.
-          { eapply DisjList_SubList; [eassumption|].
-            apply DisjList_comm, tree2Topo_minds_merss_disj.
+    - clear H2.
+      red; intros.
+      destruct H2.
+      apply MsgsP_other_midx_deqMsgs_inv in H3.
+      + specialize (H (conj H2 H3)); dest.
+        split.
+        * red; intros.
+          specialize (H _ H5).
+          destruct (oss@[oidx]) as [ost|] eqn:Host; simpl in *; auto.
+          destruct H.
+          { left.
+            red in H; dest.
+            repeat split; [assumption..|].
+            apply MsgsP_deqMsgs; assumption.
           }
-          { eapply tree2Topo_obj_chns_minds_SubList with (oidx:= oidx).
-            { specialize (H0 oidx); simpl in H0.
-              rewrite Host in H0; simpl in H0.
-              eassumption.
+          { right.
+            destruct H as [idm ?]; dest.
+            exists idm; split; [|assumption].
+            apply deqMsgs_InMP_midx; [assumption|].
+            destruct H1.
+            eapply DisjList_In_1.
+            { eapply DisjList_SubList; [eassumption|].
+              apply DisjList_comm, tree2Topo_minds_merss_disj.
             }
-            { inv H6; rewrite H9.
-              solve_SubList.
+            { eapply tree2Topo_obj_chns_minds_SubList with (oidx:= oidx).
+              { specialize (H0 oidx); simpl in H0.
+                rewrite Host in H0; simpl in H0.
+                eassumption.
+              }
+              { inv H6; rewrite H9.
+                solve_SubList.
+              }
             }
           }
-      + apply MsgsP_deqMsgs; assumption.
+        * apply MsgsP_deqMsgs; assumption.
 
-    - destruct H1.
-      simpl; eapply DisjList_SubList; [eassumption|].
-      eapply DisjList_comm, DisjList_SubList.
-      + eapply SubList_trans;
-          [|eapply tree2Topo_obj_chns_minds_SubList with (oidx:= eidx)].
-        * solve_SubList.
-        * specialize (H0 eidx); simpl in H0.
-          rewrite Heost in H0; simpl in H0.
-          eassumption.
-      + apply tree2Topo_minds_merss_disj.
+      + destruct H1.
+        simpl; eapply DisjList_SubList; [eassumption|].
+        eapply DisjList_comm, DisjList_SubList.
+        * eapply SubList_trans;
+            [|eapply tree2Topo_obj_chns_minds_SubList with (oidx:= eidx)].
+          { solve_SubList. }
+          { specialize (H0 eidx); simpl in H0.
+            rewrite Heost in H0; simpl in H0.
+            eassumption.
+          }
+        * apply tree2Topo_minds_merss_disj.
+
+    - clear H.
+      red; intros.
+      specialize (H2 H).
+      red; intros.
+      specialize (H2 _ H3).
+      destruct (oss@[oidx]) as [ost|] eqn:Host; simpl in *; auto.
+      destruct H2.
+      + left.
+        red in H2; dest.
+        repeat split; [assumption..|].
+        apply MsgsP_deqMsgs; assumption.
+      + right.
+        destruct H2 as [idm ?]; dest.
+        exists idm; split; [|assumption].
+        apply deqMsgs_InMP_midx; [assumption|].
+        destruct H1.
+        eapply DisjList_In_1.
+        { eapply DisjList_SubList; [eassumption|].
+          apply DisjList_comm, tree2Topo_minds_merss_disj.
+        }
+        { eapply tree2Topo_obj_chns_minds_SubList with (oidx:= oidx).
+          { specialize (H0 oidx); simpl in H0.
+            rewrite Host in H0; simpl in H0.
+            eassumption.
+          }
+          { inv H4; rewrite H7.
+            solve_SubList.
+          }
+        }
   Qed.
 
-  Corollary mesi_InvExcl_InvTrsOuts: InvTrsOuts impl InvExcl.
+  Corollary mesi_InvExcl_InvTrsOuts: InvTrsOuts impl (InvExcl topo).
   Proof.
     red; intros.
     inv H1.
@@ -326,21 +432,33 @@ Section InvExcl.
   Lemma mesi_InvExcl_InvTrs_init:
     forall st1,
       Reachable (steps step_m) impl st1 ->
-      InvExcl st1 ->
+      InvExcl topo st1 ->
       forall oidx ridx ins outs st2,
         SubList (idsOf ins) (sys_merqs impl) ->
         step_m impl st1 (RlblInt oidx ridx ins outs) st2 ->
         AtomicInv
           InvExclMsgOutPred
           ins st1 [RlblInt oidx ridx ins outs] outs st2 /\
-        InvExcl st2.
+        InvExcl topo st2.
   Proof.
   Admitted.
+
+  Ltac disc_bind_true :=
+    repeat
+      match goal with
+      | |- _ <+- ?ov; _ =>
+        first [match goal with
+               | [H: ov = _ |- _] => rewrite H in *; simpl in *
+               end
+              |let Hov := fresh "H" in
+               let v := fresh "v" in
+               destruct ov as [v|] eqn:Hov; simpl in *; [|auto]]
+      end.
 
   Ltac disc_rule_custom ::=
     try disc_AtomicInv.
 
-  Lemma mesi_InvExcl_InvTrs: InvTrs impl InvExcl.
+  Lemma mesi_InvExcl_InvTrs: InvTrs impl (InvExcl topo).
   Proof.
     eapply inv_atomic_InvTrs;
       [red; intros; eapply mesi_InvExcl_InvTrsIns; eauto
@@ -366,6 +484,8 @@ Section InvExcl.
     (*               msiSv_impl_ORqsInit *)
     (*               msiSv_impl_GoodRqRsSys *)
     (*               msiSv_impl_RqRsDTree Hr1) as Hpulinv. *)
+    pose proof (mesi_MsgConflictsInv
+                  (@mesi_RootChnInv_ok _ Htr) Hr1) as Hpmcf.
 
     specialize (IHAtomic H1 _ H9); dest.
     inv_step.
@@ -395,6 +515,39 @@ Section InvExcl.
           by (apply subtreeChildrenIndsOf_parentIdxOf; auto).
 
         dest_in.
+
+        { (* [liGetSImmS] *)
+          disc_rule_conds_ex.
+          split.
+          { admit. }
+          { red; simpl; intros; mred; simpl.
+            { (* "this" updated *)
+              admit.
+            }
+            { (* others *)
+              
+              (* red; intros. *)
+              (* disc_ObjExcl0_msgs H11. *)
+
+              (* eapply ObjExcl0_other_msg_id_deqMP_inv in H11. *)
+              (* 2: eassumption. *)
+              (* 2: simpl; rewrite H12; discriminate. *)
+
+              (* specialize (H6 H11); dest. *)
+
+              (* assert (NoRsI oidx msgs). *)
+              (* { solve_NoRsI_base. *)
+              (*   solve_NoRsI_by_no_uplock oidx. *)
+              (* } *)
+
+              (** TODO: develop lemmas to draw contradiction
+               * using [ObjsInvalid], state of [oidx], and [NoRsI].
+               *)
+              admit.
+            }
+          }
+        }
+        
         all: admit.
       }
 
@@ -445,7 +598,7 @@ Section InvExcl.
   Qed.
 
   Lemma mesi_InvExcl_step:
-    InvStep impl step_m InvExcl.
+    InvStep impl step_m (InvExcl topo).
   Proof.
     apply invSeq_serializable_invStep.
     - apply mesi_InvExcl_init.
@@ -457,7 +610,7 @@ Section InvExcl.
   Qed.
 
   Lemma mesi_InvExcl_ok:
-    Invariant.InvReachable impl step_m InvExcl.
+    Invariant.InvReachable impl step_m (InvExcl topo).
   Proof.
     apply inv_reachable.
     - apply mesi_InvExcl_init.
